ntor/Security.ec
@@ -1,17 +1,107 @@
-require import AllCore FSet FMap Distr NTOR Games.
+require import AllCore FSet FMap Distr List NTOR Games.
 import GAKEc.
+require Birthday.
+
 
 (* ------------------------------------------------------------------------------------------ *)
 (* Reductions *)
 (* ------------------------------------------------------------------------------------------ *)
 
+ module RO_h = {
+  var cache : (pkey * pkey * s_id * pkey * pkey, tag * key) fmap 
+
+  proc init(): unit = {
+    cache <- empty;
+  }
+
+  proc get(x: pkey * pkey * s_id * pkey * pkey) : tag * key = {
+    var t, k;
+
+    t <$ dtag;
+    k <$ dkey;
+    if (x \notin cache) {
+      cache.[x] <- (t, k);
+    }
     
+    return oget cache.[x];
+  }
+}.
+
+
+(* ------------------------------------------------------------------------------------------ *)
+(* Ctxt Collision Reduction *)
+
+op q_is : { int | 0 <= q_is } as ge0_q_is.
+op q_m1 : { int | 0 <= q_m1 } as ge0_q_m1.
+op q_m2 : { int | 0 <= q_m2 } as ge0_q_m2.
+clone Birthday as BB with
+  type T  <- (pkey * skey),
+  op   uT <- dkp,
+  op q <- q_is + q_m1 + q_m2
+  proof*.
+realize ge0_q by smt(ge0_q_is ge0_q_m1 ge0_q_m2).
+
+module Counter (G : GAKE_out) : GAKE_out_i = {
+  var cis, cm1, cm2 : int
+
+  include G[h, set_cert, send_msg3, c_rev_skey, s_rev_skey, rev_ltkey, c_rev_ephkey, s_rev_ephkey, c_test, s_test]
+
+  proc init_mem() = {
+    (cis, cm1, cm2) <- (0, 0, 0);
+  }
+  
+  proc init_s(x) = {
+    var m;
+    cis <- cis + 1;
+    m <@ G.init_s(x);
+    return m;
+  }
+  proc send_msg1(x) = {
+    var m;
+    cm1 <- cm1 + 1;
+    m <@ G.send_msg1(x);
+    return m;
+  }
+  proc send_msg2(x) = {
+    var m;
+    cm2 <- cm2 + 1;
+    m <@ G.send_msg2(x);
+    return m;
+  }
+}.
+
+module Red_Coll_O_AKE (S : BB.ASampler) = Game0 with {
+  proc init_s [
+    ^if.^kp<$ ~ {kp <@ S.s();}
+  ]
+
+  proc send_msg1 [
+    ^if.^match#None.^kp<$ ~ {kp <@ S.s();}
+  ]
+
+  proc send_msg2 [
+    ^match#Some.^match#None.^kp<$ ~ { kp <@ S.s(); }
+  ]
+}.
+
+module (Red_Coll (A : A_GAKE) : BB.Adv) (S : BB.ASampler) = {
+  proc a() = {
+    var b;
+    Red_Coll_O_AKE(S).init_mem();
+    Counter(Red_Coll_O_AKE(S)).init_mem();
+    b <@ A(Counter(Red_Coll_O_AKE(S))).run();
+  }
+}.
+
+
+
+
 (* ------------------------------------------------------------------------------------------ *)
 (* Security Proof *)
 (* ------------------------------------------------------------------------------------------ *)
 section.
 
-declare module A <: A_GAKE {-GAKE0, -Game0, -Game1}.
+declare module A <: A_GAKE {-GAKE0, -RO_h, -Game0, -Game1, -Red_Coll, -BB.Sample }.
 
 declare axiom A_ll (G <: GAKE_out{-A}):
   islossless G.h =>
@@ -29,46 +119,55 @@ declare axiom A_ll (G <: GAKE_out{-A}):
   islossless G.s_test =>
   islossless A(G).run.
 
+declare axiom A_bounded_qs: forall (G <: GAKE_out{-A}), hoare[A(Counter(G)).run: Counter.cis = 0 /\ Counter.cm1 = 0 /\ Counter.cm2 = 0 ==> Counter.cis <= q_is /\ Counter.cm1 <= q_m1 /\ Counter.cm2 <= q_m2].
+
+
 lemma Step0 &m :
-  Pr[E_GAKE(GAKE0(NTOR_S, NTOR_C), A).run() @ &m : res] = Pr[E_GAKE(Game0, A).run() @ &m : res].
+  Pr[E_GAKE(GAKE0(NTOR_S(RO_h), NTOR_C(RO_h), RO_h), A).run() @ &m : res] = Pr[E_GAKE(Game0, A).run() @ &m : res].
 proof. 
 byequiv => //.
 proc; inline*.
-sim (: ={servers, c_smap, s_smap}(GAKE0, Game0)).
+call (: ={servers, c_smap, s_smap}(GAKE0, Game0) /\ RO_h.cache{1} = Game0.hm{2}); 1,3,7,8,9,10,11,12,13: by sim />.
 
-- proc; inline*; auto=> /> &2.
-  by case: (Game0.c_smap.[i]{2})=> /> [] />.
-
-- proc; inline*.
-  sp; match = => // sk.
-  match = => //.
-  match Some {1} 4.
-  + by auto=> /> _ _ _ _; exists (b{m0}, sk, None).
-  match Some {1} 10=> //; 1: by auto=> /> /#.
-  by auto.
+- proc; inline*; auto; if => //; auto => /#.
 
 - proc; inline*. 
   sp; if => //.
   sp; match = => // [|st]; 1:by auto.
   by match = => // st' pt' ir'; auto.
 
-- by proc; inline*; if => //; auto=> /#.
+- proc; inline*.
+  sp; match = => // sk.
+  match = => //.
+  match Some {1} 4.
+  + by auto=> /> _ _ _ _; exists (b{m0}, sk, None).
+  match Some {1} 14=> //; 1: by auto=> /> /#.
+  by auto => />.
+
+- proc; inline*; auto=> />.
+  sp; match = => //; 1: auto.
+  by match = => //; 1: auto.
+
+by auto.
 qed.
 
-lemma Step1 &m: `| Pr[E_GAKE(Game0, A).run() @ &m : res] - Pr[E_GAKE(Game1, A).run() @ &m : res] | <= Pr[E_GAKE(Game1, A).run() @ &m : Game1.bad].
+lemma Step1 &m: `| Pr[E_GAKE(Game0, A).run() @ &m : res] - Pr[E_GAKE(Game1, A).run() @ &m : res] | <= Pr[E_GAKE(Game0, A).run() @ &m : Game0.bad].
 proof.
-byequiv (: _ ==> _) : Game0.bad => //; first last.
+rewrite StdOrder.RealOrder.distrC.
+byequiv (: _ ==> _) : Game1.bad => //; first last.
 + by rewrite eq_iff.
-proc; inline*.
+symmetry; proc; inline*.
 call (: Game1.bad
-      , ={servers, c_smap, s_smap, kp_set, bad}(Game0, Game1)
+      , ={servers, c_smap, s_smap, kp_set, hm, outs_h, bad, bad_ro}(Game0, Game1)
       , ={bad}(Game0, Game1)) => //. 
 
 - exact A_ll.
 
 - by proc; auto.
-- by move => &2 bad; proc; auto.
-- by move => &1; proc; auto.
+- move => &2 bad; proc; auto => />. 
+  by rewrite dkey_ll dtag_ll.
+- move => &1; proc; auto.
+  by rewrite dkey_ll dtag_ll.
 
 - proc.
   if => //.
@@ -108,97 +207,168 @@ call (: Game1.bad
   + by rewrite dkp_ll.
   by smt().
 
-- proc.
+- proc; inline*.
   sp; match = => //. 
   move => sk.
   match = => //.
   + seq 1 1: (#pre /\ ={kp}); 1: by auto.
-    by sp 0 1; if{2}; auto => />.
+  sp 0 1; if{2}.
+  + by auto => />. 
+  auto.
 - move => &2 bad.
-  proc; sp; match; auto => />.
+  proc; inline*; sp; match; auto => />.
   match; auto => />.
-  rewrite dkp_ll. 
+  rewrite dkp_ll dkey_ll dtag_ll. 
   by smt().
 - move => &1. 
   proc; sp; match; auto => />.
-  match; auto => />.
+  match; 2: by auto => />. 
+  rcondf ^if; 1: by auto => />. 
+  auto => />.
   by rewrite dkp_ll.
 
-- proc; auto => />. 
-  by smt().
+- sim />.
 - move => &2 bad.
-  proc; auto => />.
-  by smt().
+  proc; inline*.
+  sp; match; auto. 
+  match; auto => />.
+  by rewrite dkey_ll dtag_ll.
 - move => &1.
-  proc; auto => />.
-  by smt().
+  proc; inline*; auto => />.
+  sp; match; auto.
+  match; auto.
+  by rewrite dkey_ll dtag_ll.
 
-- proc; auto => />. 
-  by smt().
+- sim />.
 - move => &2 bad.
-  proc; auto => />.
-  by smt().
+  proc; sp; match; 1: by auto. 
+  match; auto => />.
 - move => &1.
-  proc; auto => />.
-  by smt().
+  proc; sp; match; 1: by auto. 
+  match; auto => />.
 
-- proc; auto => />. 
-  by smt().
+- sim />.
 - move => &2 bad.
-  proc; auto => />.
-  by smt().
+  proc; sp; match; 1: by auto. 
+  match; auto => />.
 - move => &1.
-  proc; auto => />.
-  by smt().
+  proc; sp; match; 1: by auto. 
+  match; auto => />.
 
-- proc; auto => />. 
-  by smt().
+- sim />.
 - move => &2 bad.
-  proc; auto => />.
-  by smt().
+  proc; sp; match; 1: by auto. 
+  match; auto => />.
 - move => &1.
-  proc; auto => />.
-  by smt().
+  proc; sp; match; 1: by auto. 
+  match; auto => />.
 
-- proc; auto => />. 
-  by smt().
+- sim />.
 - move => &2 bad.
-  proc; auto => />.
-  by smt().
+  proc; sp; match; 1: by auto. 
+  match; auto => />.
 - move => &1.
-  proc; auto => />.
-  by smt().
+  proc; sp; match; 1: by auto. 
+  match; auto => />.
 
-- proc; auto => />. 
-  by smt().
+- sim />.
 - move => &2 bad.
-  proc; auto => />.
-  by smt().
+  proc; sp; match; 1: by auto. 
+  match; auto => />.
 - move => &1.
-  proc; auto => />.
-  by smt().
+  proc; sp; match; 1: by auto. 
+  match; auto => />.
 
-- proc; auto => />. 
-  by smt().
+- sim />.
 - move => &2 bad.
-  proc; auto => />.
-  by smt().
+  proc; sp; match; 1: by auto. 
+  match; auto => />.
 - move => &1.
-  proc; auto => />.
-  by smt().
+  proc; sp; match; 1: by auto. 
+  match; auto => />.
 
-- proc; auto => />. 
-  by smt().
+- sim />.
 - move => &2 bad.
-  proc; auto => />.
-  by smt().
+  proc; sp; match; 1: by auto. 
+  match; auto => />.
 - move => &1.
-  proc; auto => />.
-  by smt().
+  proc; sp; match; 1: by auto. 
+  match; auto => />.
 
 auto => />.
-move => rl rr al bl dl pl kpl sl ar br dr pr kpr sr. 
+move => rl rr al bl brl csl hml kpl hsl ssl sl ar br brr csr hmr kpr hsr ssr sr. 
 by case : (!br) => />.
 qed.
 
+
+(* ------------------------------------------------------------------------------------------ *)
+(* Step 1b: Bound the bad event. *)
+lemma Step1b &m: Pr[E_GAKE(Game0, A).run() @ &m : Game0.bad] <= ((q_is + q_m1 + q_m2) ^ 2)%r * mu1 dkp (mode dkp).
+proof.
+apply (StdOrder.RealOrder.ler_trans Pr[BB.Exp(BB.Sample, Red_Coll(A)).main() @ &m : ! uniq BB.Sample.l]); first last.
++ apply (BB.pr_collision_q2 (Red_Coll(A))).
+  + move => S S_ll.
+    islossless.
+    apply (A_ll (Counter(Red_Coll_O_AKE(S)))); islossless.
+    + match; 1: auto; islossless.
+      match; auto.
+    + match; auto. 
+      by sp; match; auto; islossless.
+    + match => //.
+      by sp; match; auto; islossless.
+    + match => //; islossless.
+      by match; islossless.
+    + by match; 1: auto; match; islossless.
+    + by match; 1: auto; match; islossless.
+    + by match; 1: auto; match; islossless.
+    + by match; 1: auto; match; islossless.
+    + by match; 1: auto; match; islossless.
+    + by match; 1: auto; match; islossless.
+  proc; inline.
+  sp.
+  conseq (: _ ==> size BB.Sample.l <= Counter.cis + Counter.cm1 + Counter.cm2) (: Counter.cis = 0 /\ Counter.cm1 = 0 /\ Counter.cm2 = 0 ==> Counter.cis <= q_is /\ Counter.cm1 <= q_m1 /\ Counter.cm2 <= q_m2)=> //.
+  + smt().
+  + by call (A_bounded_qs (Red_Coll_O_AKE(BB.Sample))).
+  call (: size BB.Sample.l <= Counter.cis + Counter.cm1 + Counter.cm2) => //.
+  + by proc; auto.
+  + by proc; inline; sp; if => //; auto => /#.
+  + by proc; auto.
+  + proc; inline; sp; if => //; 2: auto => /#.
+    by sp; match; auto => /#.
+  + proc; inline; sp; match; 1: auto => /#.
+    case ((Red_Coll_O_AKE.s_smap.[b, j]) = None).
+    + by match None ^match; auto => /#.
+    by match Some ^match; auto => /#.
+  + by proc; inline; sp; match; 1: auto; match; auto => /#.
+  + by proc; sp; match; 1: auto; match; auto => /#.
+  + by proc; sp; match; 1: auto; match; auto => /#.
+  + by proc; sp; match; 1: auto; match; auto => /#.
+  + by proc; sp; match; 1: auto; match; auto => /#.
+  + by proc; sp; match; 1: auto; match; auto => /#.
+  + by proc; sp; match; 1: auto; match; auto => /#.
+  + by proc; sp; match; 1: auto; match; auto => /#.
+  auto => /#.
+byequiv => //.
+proc; inline.
+call (:
+ ={hm, outs_h, servers, c_smap, s_smap, kp_set, bad, bad_ro}(Game0, Red_Coll_O_AKE(BB.Sample))
+ /\ (Game0.bad{1} => !uniq BB.Sample.l{2})
+ /\ (forall kp, kp \in Game0.kp_set{1} <=> kp \in BB.Sample.l{2})
+) => //; 1,3,6,7,8,9,10,11,12,13: by sim />.
++ proc; inline; sp 0 2; if => //; auto => />. 
+  move => &2 H I J K L.
+  split. smt(mem_set).
+  
+  admit.
++ admit. 
++ admit. 
+auto => />.
+smt(in_fset0).
+qed.
+
+
 end section.
+
+
+
+
